\documentclass{article}
\usepackage{amsmath,amssymb,newlfont,graphicx,caption,verbatim}
\newcommand{\dom}{\mathrm{dom}}
\newcommand{\len}{\mathit{len}}
\newcommand{\poly}{\mathsf{poly}}
\newcommand{\flow}{\mathsf{flow}}
\newcommand{\jump}{\mathsf{jump}}
\newcommand{\inv}{\mathsf{inv}}
\newcommand{\init}{\mathsf{init}}
\newcommand{\guard}{\mathsf{guard}}
\newcommand{\reset}{\mathsf{reset}}
\newcommand{\reach}{\mathsf{Reach}}
\newcommand{\unsafe}{\mathsf{unsafe}}
\newcommand{\safe}{\mathsf{safe}}

\title{A Power Grid Model}
\author{}
\begin{document}
\maketitle

The model~\cite{source} is defined as follows. 

\paragraph{Mode 1 (fault-on)}
The $\flow_1$ condition:
\begin{eqnarray*}
d\delta_1/dt &=& \omega_1\\
d\delta_2/dt &=& \omega_2\\
d\omega_1/dt &=& \frac{\omega_s}{2H_1a}(P_{m1} - D\omega_1 - P_{e1}^1(x))\\
d\omega_2/dt &=& \frac{\omega_s}{2H_1a}(P_{m2} - D\omega_2 - P_{e2}^1(x))\\
dz/dt &=& 1
\end{eqnarray*}
where
\begin{eqnarray*}
P_{e1}^1 &=& G_{11}^1V_i^2 + \Big(G_{11}^1 V_1V_2\cos(\delta_1-\delta_2) +
B_{12}^1 V_1V_2\sin(\delta_1-\delta_2)\\
&+& G_{1\infty}^1
V_1V_{\infty}\cos(\delta_1-\delta_{\infty}) + B_{1\infty}^1
V_1V_{\infty}\sin(\delta_1-\delta_{\infty}) \Big)\\
P_{e2}^1 &=& G_{11}^1V_i^2 + \Big(G_{11}^1 V_1V_2\cos(\delta_1-\delta_2) +
B_{12}^1 V_1V_2\sin(\delta_1-\delta_2)\\
&+& G_{1\infty}^1
V_1V_{\infty}\cos(\delta_1-\delta_{\infty}) + B_{1\infty}^1
V_1V_{\infty}\sin(\delta_1-\delta_{\infty}) \Big)
\end{eqnarray*}
The jump condition $\jump_{1 \rightarrow 2}:$
$$z = t_cl.$$

\paragraph{Mode 2 (1 line operation)}
The $\flow_2$ condition:
\begin{eqnarray*}
d\delta_1/dt &=& \omega_1\\
d\delta_2/dt &=& \omega_2\\
d\omega_1/dt &=& \frac{\omega_s}{2H_1a}(P_{m1} - D\omega_1 - P_{e1}^1(x))\\
d\omega_2/dt &=& \frac{\omega_s}{2H_1a}(P_{m2} - D\omega_2 - P_{e2}^1(x))\\
dz/dt &=& 1
\end{eqnarray*}
where
\begin{eqnarray*}
P_{e1}^2 &=& G_{22}^1V_2^2 + \Big(G_{22}^1 V_1V_2\cos(\delta_2-\delta_1) +
B_{21}^2 V_1V_2\sin(\delta_2-\delta_1)\\
&+& G_{2\infty}^2
V_2V_{\infty}\cos(\delta_2-\delta_{\infty}) + B_{2\infty}^1
V_2V_{\infty}\sin(\delta_2-\delta_{\infty}) \Big)\\
P_{e2}^2 &=& G_{22}^1V_2^2 + \Big(G_{22}^1 V_1V_2\cos(\delta_2-\delta_1) +
B_{21}^2 V_1V_2\sin(\delta_2-\delta_1)\\
&+& G_{2\infty}^2
V_2V_{\infty}\cos(\delta_2-\delta_{\infty}) + B_{2\infty}^1
V_2V_{\infty}\sin(\delta_2-\delta_{\infty}) \Big)
\end{eqnarray*}
The jump condition $\jump_{2 \rightarrow 3}:$
$$z_2(x) = 0 \wedge d(z2)/dt < 0.$$
where
\begin{eqnarray*}
z2 &=& \frac{V_2}{|I_2^(2)|^2}\Big( \cos\delta_2 \sum_{j\in
\{1,2,\infty\}}V_j(G_{2j}^{(2)}\cos\delta_j - B_{2j}^{2}\sin \delta_j)\\
&+&\sin \delta_2 \sum_{j\in \{1,2,\infty\}}V_j(G_{2j}^{(2)}\sin \delta_j +
B_{2j}^{(2)}\cos\delta_j )\Big).
\end{eqnarray*}


\paragraph{Mode 3 ()}
The $\flow_1$ condition:
\begin{eqnarray*}
d\delta_1/dt &=& \omega_1\\
d\delta_2/dt &=& \omega_2\\
d\omega_1/dt &=& \frac{\omega_s}{2H_1a}(P_{m1} - D\omega_1 - P_{e1}^1(x))\\
d\omega_2/dt &=& \frac{\omega_s}{2H_1a}(P_{m2} - D\omega_2 - P_{e2}^1(x))\\
dz/dt &=& 1
\end{eqnarray*}
where
\begin{eqnarray*}
P_{e1}^1 &=& G_{11}^1V_i^2 + \Big(G_{11}^1 V_1V_2\cos(\delta_1-\delta_2) +
B_{12}^1 V_1V_2\sin(\delta_1-\delta_2)\\
&+& G_{1\infty}^1
V_1V_{\infty}\cos(\delta_1-\delta_{\infty}) + B_{1\infty}^1
V_1V_{\infty}\sin(\delta_1-\delta_{\infty}) \Big)\\
P_{e2}^1 &=& G_{11}^1V_i^2 + \Big(G_{11}^1 V_1V_2\cos(\delta_1-\delta_2) +
B_{12}^1 V_1V_2\sin(\delta_1-\delta_2)\\
&+& G_{1\infty}^1
V_1V_{\infty}\cos(\delta_1-\delta_{\infty}) + B_{1\infty}^1
V_1V_{\infty}\sin(\delta_1-\delta_{\infty}) \Big)
\end{eqnarray*}
The jump condition $\jump_{1 \rightarrow 2}:$
$$z = t_cl.$$


\paragraph{Mode 4 ()}
The $\flow_1$ condition:
\begin{eqnarray*}
d\delta_1/dt &=& \omega_1\\
d\delta_2/dt &=& \omega_2\\
d\omega_1/dt &=& \frac{\omega_s}{2H_1a}(P_{m1} - D\omega_1 - P_{e1}^1(x))\\
d\omega_2/dt &=& \frac{\omega_s}{2H_1a}(P_{m2} - D\omega_2 - P_{e2}^1(x))\\
dz/dt &=& 1
\end{eqnarray*}
where
\begin{eqnarray*}
P_{e1}^1 &=& G_{11}^1V_i^2 + \Big(G_{11}^1 V_1V_2\cos(\delta_1-\delta_2) +
B_{12}^1 V_1V_2\sin(\delta_1-\delta_2)\\
&+& G_{1\infty}^1
V_1V_{\infty}\cos(\delta_1-\delta_{\infty}) + B_{1\infty}^1
V_1V_{\infty}\sin(\delta_1-\delta_{\infty}) \Big)\\
P_{e2}^1 &=& G_{11}^1V_i^2 + \Big(G_{11}^1 V_1V_2\cos(\delta_1-\delta_2) +
B_{12}^1 V_1V_2\sin(\delta_1-\delta_2)\\
&+& G_{1\infty}^1
V_1V_{\infty}\cos(\delta_1-\delta_{\infty}) + B_{1\infty}^1
V_1V_{\infty}\sin(\delta_1-\delta_{\infty}) \Big)
\end{eqnarray*}
The jump condition $\jump_{1 \rightarrow 2}:$
$$z = t_cl.$$


\paragraph{Constants} The constants that are used in the description have the
following values. 
\begin{align*}
\alpha_x = 0.0204 && \alpha_y = 0.0242 && \beta_x = 0.0076 && \beta_y = 0.0168
\\
k_1 = 0 && k_2 = 2 && k_3 = 0.8 && k_4 = 0.5 \\
d\in [0,1] && m_1 = 5\times 10^{-5} && z_0 = 20 && \tau = 62.5 \\
r_1 = 10 && r_0 = 4
\end{align*}
\paragraph{Properties}
The following properties can be checked on the model. 


\begin{thebibliography}{1}
\bibitem{source} Yoshihiko Susuki, T. John Koo, Hiroaki Ebina, Takuya Yamazaki,
Takashi Ochi, Takuji Uemura, and Takashi Hikihara. {\em A Hybrid System
Approach to the Analysis and Design of Power Grid Dynamic Peformance.}
Proceedings of the IEEE, Vol 100, No.1, 2012.


  \end{thebibliography}


\end{document}
